new/proof/github_com/goose_lang/goose/model/channel/idiom/base.v
@@ -1,19 +1,19 @@
 From New.proof.github_com.goose_lang.goose.model.channel Require Export chan_au_base.
 From Perennial.algebra Require Import auth_set.
+From iris.algebra.lib Require Import dfrac_agree.
 From iris.base_logic Require Import ghost_map.
 From iris.base_logic.lib Require Import saved_prop.
 From Perennial.algebra Require Export ghost_var.
 
 Class chan_idiomG Σ V := ChanIdiomG {
     chan_idiom_chanG :: chanG Σ V;
-    chan_idiom_ghost_mapG :: ghost_mapG Σ nat gname;
-    (* already in chanG *)
-    (* chan_idiom_savedPropG :: savedPropG Σ; *)
-    chan_idiom_ghost_boolG :: ghost_varG Σ bool;
-    chan_idiom_ghost_listG :: ghost_varG Σ (list V);
-    chan_idiom_setG :: auth_setG Σ gname;
-    chan_idiom_ghost_natG :: ghost_varG Σ nat;
-    chan_idiom_ghost_unitG :: ghost_varG Σ ();
+    #[local] chan_idiom_ghost_mapG :: ghost_mapG Σ nat gname;
+    #[local] chan_idiom_ghost_boolG :: ghost_varG Σ bool;
+    #[local] chan_idiom_ghost_listG :: ghost_varG Σ (list V);
+    #[local] chan_idiom_setG :: auth_setG Σ gname;
+    #[local] chan_idiom_ghost_natG :: ghost_varG Σ nat;
+    #[local] chan_idiom_ghost_unitG :: ghost_varG Σ ();
+    #[local] chan_idiom_closeable_tok_inG :: inG Σ (dfrac_agreeR boolO);
 }.
 
 Definition chan_idiomΣ V : gFunctors :=
